Big cleaning in translations

translations/translation_utils.v
@@ -1,29 +1,10 @@
-From Template Require Import Ast Typing Checker LiftSubst monad_utils Template.
-Require Import Translations.sigma.
+From Template Require Import Ast Typing Checker LiftSubst monad_utils utils Template.
 Require Import List.
 Import ListNotations MonadNotation String.
 Open Scope string_scope.
 
 Axiom todo : forall {A}, A.
 
-
-Hint Resolve String.string_dec Peano_dec.eq_nat_dec : eq_dec.
-
-Definition string_of_gref gr :=
-  match gr with
-  | ConstRef s => s
-  | IndRef (mkInd s n) => "todo" ++ s
-  | ConstructRef (mkInd s n) k => "todo" ++ s
-  end.
-
-Definition gref_eq_dec
-  : forall gr gr' : global_reference, {gr = gr'} + {~ gr = gr'}.
-  decide equality; eauto with eq_dec.
-  destruct i, i0.
-  decide equality; eauto with eq_dec.
-  destruct i, i0.
-  decide equality; eauto with eq_dec.
-Defined.
 
 Definition tsl_table := list (global_reference * term).
 
@@ -39,6 +20,7 @@ Fixpoint lookup_tsl_table (E : tsl_table) (gr : global_reference)
 
 Definition tsl_context := (global_context * tsl_table)%type.
 
+Definition emptyTC : tsl_context := ([], []).
 
 Inductive tsl_error :=
 | NotEnoughFuel
@@ -76,7 +58,7 @@ Instance monad_exc : MonadExc tsl_error tsl_result :=
 Class Translation := { tsl_id : ident -> ident ;
                        tsl_tm : tsl_context -> term -> tsl_result term ;
                        tsl_ty : tsl_context -> term -> tsl_result term ;
-                       tsl_ind : tsl_context -> ident -> minductive_decl
+                       tsl_ind : tsl_context -> kername -> kername -> minductive_decl
                             -> tsl_result (tsl_table * list minductive_decl)
                      }.
 
@@ -90,185 +72,51 @@ Definition tsl_name tsl_ident n :=
   end.
 
 
-Quote Definition tSigma := sigma.
-Quote Definition tPair := @mk_sig.
-Definition pair (typ1 typ2 t1 t2 : term) : term
-  := tApp tPair [ typ1 ; typ2 ; t1 ; t2].
-Definition pack (t u : term) : term
-  := tApp tSigma [ t ; u ].
-Definition proj1 (t : term) : term
-  := tProj (mkInd "Translations.sigma.sigma" 0, 2, 0) t.
-Definition proj2 (t : term) : term
-  := tProj (mkInd "Translations.sigma.sigma" 0, 2, 1) t.
-Definition proj (b : bool) (t : term) : term
-  := tProj (mkInd "Translations.sigma.sigma" 0, 2, if b then 0 else 1) t.
 
-Quote Definition tBool := bool.
-Quote Definition tTrue := true.
-Definition timesBool (t : term) :=
-  tApp tSigma [t; tLambda nAnon t tBool].
-Definition pairTrue typ t := pair typ (tLambda nAnon typ tBool) t tTrue.
-
-
-
-Definition print_nf {A} (msg : A) : TemplateMonad unit
-  := (tmEval all msg) >>= tmPrint.
-
-Definition fail_nf {A} (msg : string) : TemplateMonad A
-  := (tmEval all msg) >>= tmFail.
-
-
-Fixpoint extract_mind_decl_from_program (id : ident) (p : program)
-  : option minductive_decl
-  := match p with
-     | PConstr _ _ _ _ p => extract_mind_decl_from_program id p
-     | PType id' n inds p => if string_dec id id' then
-                              Some (Build_minductive_decl n inds)
-                            else extract_mind_decl_from_program id p
-     | PAxiom _ _ _ p => extract_mind_decl_from_program id p
-     | PIn _ => None
-     end.
-
-Fixpoint decompose_prod (t : term) : (list name) * (list term) * term :=
-  match t with
-  | tProd n A B => let (nAs, B) := decompose_prod B in
-                  let (ns, As) := nAs in
-                  (n :: ns, A :: As, B)
-  | _ => ([], [], t)
-  end.
-
-Definition get_ident (n : name) :=
-  match n with
-  | nAnon => "XX"
-  | nNamed i => i
-  end.
-
-Fixpoint remove_arity (n : nat) (t : term) : term :=
-  match n with
-  | O => t
-  | S n => match t with
-          | tProd _ _ B => remove_arity n B
-          | _ => t (* todo *)
-          end
-  end.
-
-Definition option_get {A} (default : A) (x : option A) : A
-  := match x with
-     | Some x => x
-     | None => default
-     end.
-
-Definition mind_decl_to_entry (decl : minductive_decl)
-  : mutual_inductive_entry.
-Proof.
-  refine {| mind_entry_record := None; (* not a record *)
-            mind_entry_finite := Finite; (* inductive *)
-            mind_entry_params := _;
-            mind_entry_inds := _;
-            mind_entry_polymorphic := false;
-            mind_entry_private := None |}.
-  - refine (match List.hd_error decl.(ind_bodies) with
-            | Some i0 => _
-            | None => nil (* assert false: at least one inductive in a mutual block *)
-            end).
-    pose (typ := decompose_prod i0.(ind_type)).
-    destruct typ as [[names types] _].
-    apply (List.firstn decl.(ind_npars)) in names.
-    apply (List.firstn decl.(ind_npars)) in types.
-    refine (List.combine _ _).
-    exact (List.map get_ident names).
-    exact (List.map LocalAssum types).
-  - refine (List.map _ decl.(ind_bodies)).
-    intros [].
-    refine {| mind_entry_typename := ind_name;
-              mind_entry_arity := remove_arity decl.(ind_npars) ind_type;
-              mind_entry_template := false;
-              mind_entry_consnames := _;
-              mind_entry_lc := _;
-            |}.
-    refine (List.map (fun x => fst (fst x)) ind_ctors).
-    refine (List.map (fun x => remove_arity decl.(ind_npars)
-                                                (snd (fst x))) ind_ctors).
-Defined.
-
-
-
-Fixpoint fold_left_i_aux {A B} (f : A -> nat -> B -> A) (n0 : nat) (l : list B)
-         (a0 : A) {struct l} : A
-  := match l with
-     | [] => a0
-     | b :: l => fold_left_i_aux f (S n0) l (f a0 n0 b)
-     end.
-Definition fold_left_i {A B} f := @fold_left_i_aux A B f 0.
-
-
-Fixpoint map_i_aux {A B} (f : nat -> A -> B) (n0 : nat) (l : list A) : list B
-  := match l with
-     | [] => []
-     | x :: l => (f n0 x) :: (map_i_aux f (S n0) l)
-     end.
-Definition map_i {A B} f := @map_i_aux A B f 0.
-
-
-Fixpoint subst_app (t : term) (us : list term) : term :=
-  match t, us with
-  | tLambda _ A t, u :: us => subst_app (t {0 := u}) us
-  | _, [] => t
-  | _, _ => mkApps t us
-  end.
-
-
-Definition tTranslate (tsl : Translation) (ΣE : tsl_context) (id : ident)
+Definition tTranslate {tsl : Translation} (ΣE : tsl_context) (id : ident)
   : TemplateMonad tsl_context :=
   gr <- tmAbout id ;;
   id' <- tmEval all (tsl_id id) ;;
+  mp <- tmCurrentModPath tt ;;
+  kn' <- tmEval all (mp ++ "." ++ id') ;;
   match gr with
   | None => fail_nf (id ++ " not found")
   | Some (ConstructRef (mkInd kn n) _)
   | Some (IndRef (mkInd kn n)) =>
       d <- tmQuoteInductive id ;;
-      let d' := tsl_ind ΣE id d in
-      d' <- tmEval lazy d' ;;
+      d' <- tmEval lazy (tsl_ind ΣE kn kn' d) ;;
       match d' with
       | Error e => print_nf e ;; fail_nf ("Translation error during the translation of the inductive " ++ id)
       | Success (E, decls) =>
-        let entries := List.map mind_decl_to_entry decls in
-        monad_fold_left (fun _ e => tmMkInductive e) entries tt ;;
-        let decl := InductiveDecl kn d in
+        monad_fold_left (fun _ e => tmMkInductive' e) decls tt ;;
         print_nf  (id ++ " has been translated as " ++ id') ;;
-        ret (decl :: fst ΣE, E ++ snd ΣE)%list
+        ret (InductiveDecl kn d :: fst ΣE, E ++ snd ΣE)%list
       end
 
   | Some (ConstRef kn) =>
     e <- tmQuoteConstant kn true ;;
     match e with
     | ParameterEntry _ => fail_nf (id ++ "is an axiom, not a definition")
-
     | DefinitionEntry {| definition_entry_type := A;
                          definition_entry_body := t |} =>
       t' <- tmEval lazy (tsl_tm ΣE t) ;;
       match t' with
       | Error e => print_nf e ;; fail_nf ("Translation error during the translation of the body of " ++ id)
       | Success t' =>
-        A' <- tmEval lazy (tsl_ty ΣE A) ;;
-        match A' with
-        | Error e => print_nf e ;; fail_nf ("Translation error during the translation of the type of " ++ id)
-        | Success A' =>
-          tmMkDefinition id' t' ;;
-          let decl := {| cst_universes := [];
-                         cst_type := A; cst_body := Some t |} in
-          let Σ' := ConstantDecl kn decl :: (fst ΣE) in
-          let E' := (ConstRef kn, tConst id' []) :: (snd ΣE) in
-          print_nf  (id ++ " has been translated as " ++ id') ;;
-          ret (Σ', E')
-        end
+        tmMkDefinition id' t' ;;
+        let decl := {| cst_universes := [];
+                       cst_type := A; cst_body := Some t |} in
+        let Σ' := ConstantDecl kn decl :: (fst ΣE) in
+        let E' := (ConstRef kn, tConst kn' []) :: (snd ΣE) in
+        print_nf  (id ++ " has been translated as " ++ id') ;;
+        ret (Σ', E')
       end
     end
   end.
 
 
 
-Definition tImplement (tsl : Translation) (ΣE : tsl_context)
+Definition tImplement {tsl : Translation} (ΣE : tsl_context)
            (id : ident) (A : Type)
   : TemplateMonad (tsl_context) :=
   tA <- tmQuote A ;;
@@ -321,35 +169,3 @@ Definition tImplement (tsl : Translation) (ΣE : tsl_context)
 (*       tmReturn (Some (Σ', E')) *)
 (*     end *)
 (*   end. *)
-
-
-
-
-(* Inductive eq' (A : Set) (x : A) : A -> Prop :=  eq_refl' : eq' A x x. *)
-(* Quote Recursively Definition eq'_prog := eq'. *)
-(* Definition eq'_decl := Eval compute in *)
-(*       extract_mind_decl_from_program "Top.eq'" eq'_prog. *)
-
-Quote Recursively Definition sigma_prog := @sigma.
-Quote Recursively Definition eq_prog := @eq.
-Quote Recursively Definition nat_prog := nat.
-
-Definition eq_decl := Eval compute in
-      option_get todo (extract_mind_decl_from_program "Coq.Init.Logic.eq" eq_prog).
-Definition sigma_decl := Eval compute in
-      option_get todo (extract_mind_decl_from_program "Translations.sigma.sigma" sigma_prog).
-Definition nat_decl := Eval compute in
-      option_get todo (extract_mind_decl_from_program "Coq.Init.Datatypes.nat" nat_prog).
-
-Definition eq_entry := Eval compute in mind_decl_to_entry eq_decl.
-Definition sigma_entry := Eval compute in mind_decl_to_entry sigma_decl.
-Definition nat_entry := Eval compute in mind_decl_to_entry nat_decl.
-(* Make Inductive eq_entry. *)
-(* Make Inductive sigma_entry. *)
-
-Require Vector.
-Require Even.
-Run TemplateProgram (d <- tmQuoteInductive "Even.even" ;;
-                     print_nf d ;;
-                     let e := mind_decl_to_entry d in
-                     tmMkInductive e).
