translations/sigma.v
@@ -1,3 +1,6 @@
+Require Import Template.Ast Template.Template.
+Require Import List String. Import ListNotations.
+
 Set Primitive Projections.
 
 Record sigma A B :=
@@ -17,3 +20,18 @@ Notation "'exists' x .. y , p" := (sigma _ (fun x => .. (sigma _ (fun y => p)) .
                                   : type_scope.
 
 Notation " A × B " := (sigma A (fun _ => B)) (at level 30) : type_scope.
+
+
+Quote Definition tSigma := sigma.
+Quote Definition tPair := @mk_sig.
+Definition pair (typ1 typ2 t1 t2 : term) : term
+  := tApp tPair [ typ1 ; typ2 ; t1 ; t2].
+Definition pack (t u : term) : term
+  := tApp tSigma [ t ; u ].
+Definition sigma_ind := Eval compute in match tSigma with tInd i _ => i | _ =>  mkInd "bug: sigma not an inductive"%string 0 end.
+Definition proj1 (t : term) : term
+  := tProj (sigma_ind, 2, 0) t.
+Definition proj2 (t : term) : term
+  := tProj (sigma_ind, 2, 1) t.
+Definition proj (b : bool) (t : term) : term
+  := tProj (sigma_ind, 2, if b then 0 else 1) t.
